bedrock2/src/Examples/bsearch.v
@@ -10,10 +10,10 @@ From bedrock2 Require Import Semantics BasicC64Semantics.
 Import HList List.
 Instance spec_of_bsearch : spec_of "bsearch"%string := fun functions =>
   forall left right target xs R t m,
-    sep (array (scalar Syntax.access_size.word) (word.of_Z 8) left xs) R m ->
+    sep (array scalar (word.of_Z 8) left xs) R m ->
     WeakestPrecondition.call (fun _ => True) (fun _ => False) (fun _ _ => True) functions
       "bsearch"%string t m (left::right::target::nil)%list
-      (fun t' m' rets => t=t' /\ sep (array (scalar Syntax.access_size.word) (word.of_Z 8) left xs) R m' /\ exists i, rets = (i::nil)%list /\
+      (fun t' m' rets => t=t' /\ sep (array scalar (word.of_Z 8) left xs) R m' /\ exists i, rets = (i::nil)%list /\
       ((*sorted*)False -> True)
       ).
 
@@ -42,8 +42,8 @@ Proof.
   refine (
     tailrec (HList.polymorphic_list.cons _ (HList.polymorphic_list.cons _ HList.polymorphic_list.nil)) ("left"::"right"::"target"::nil)%list%string
         (fun l xs R t m left right target => PrimitivePair.pair.mk
-          (sep (array (scalar Syntax.access_size.word) (word.of_Z 8) left xs) R m /\ List.length xs = l)
-        (fun        T M LEFT RIGHT TARGET => T = t /\ sep (array (scalar Syntax.access_size.word) (word.of_Z 8) left xs) R M))
+          (sep (array scalar (word.of_Z 8) left xs) R m /\ List.length xs = l)
+        (fun        T M LEFT RIGHT TARGET => T = t /\ sep (array scalar (word.of_Z 8) left xs) R M))
         lt _ _ _ _ _ _ _);
     cbn [reconstruct map.putmany_of_list HList.tuple.to_list
          HList.hlist.foralls HList.tuple.foralls
