bedrock2/src/ProgramLogic.v
@@ -138,11 +138,12 @@ Ltac straightline :=
     let x := rdelta x in is_evar x; change (x=y); exact eq_refl
   | |- ?x = ?y =>
     let x := rdelta x in let y := rdelta y in constr_eq x y; exact eq_refl
-  | |- @store _ _ _ _ _ _ =>  eapply Scalars.store_sep; [solve[ecancel_assumption]|]
+  | |- @store _ _ _ _ _ _ =>  eapply Scalars.store_word_of_sep; [solve[ecancel_assumption]|]
   | |- bedrock2.Memory.load Syntax.access_size.word ?m ?a = Some ?ev =>
-    try subst ev; eapply Scalars.load_word_sep; ecancel_assumption
+    try subst ev; eapply Scalars.load_word_of_sep; ecancel_assumption
   | |- bedrock2.Memory.load _ ?m ?a = Some ?ev =>
-    try subst ev; eapply Scalars.load_sep; ecancel_assumption
+    (* TODO do we need lemmas for all load sizes? *)
+    try subst ev; eapply Scalars.load_word_of_sep; ecancel_assumption
   | |- exists x, ?P /\ ?Q =>
     let x := fresh x in refine (let x := _ in ex_intro (fun x => P /\ Q) x _);
                         split; [solve [repeat straightline]|]
